dirty tricks to get restricted funext

theories/SetModel/HO.v
@@ -121,27 +121,94 @@ Proof.
     + refine (transpS (fun X => X ⊂ _) H _). easy.
 Qed.
 
+(* Restricting the domain of higher-order functions to get funext *)
+(* Requires excluded middle! *)
+
+Definition is_clipped (Γ : ZFSet) (f : ZFSet -> ZFSet) : SProp :=
+  forall γ, (¬ γ ∈ Γ) -> f γ ≡ atom.
+
+Definition clip (Γ : ZFSet) (f : ZFSet -> ZFSet) : ZFSet -> ZFSet :=
+  fun γ => ι { x ϵ { atom ; f γ } ∣ (γ ∈ Γ ∧ x ≡ f γ) ∨ (¬ γ ∈ Γ ∧ x ≡ atom) }.
+
+Lemma clip_typing (Γ : ZFSet) (f : ZFSet -> ZFSet) (γ : ZFSet) :
+  clip Γ f γ ∈ { x ϵ { atom ; f γ } ∣ (γ ∈ Γ ∧ x ≡ f γ) ∨ (¬ γ ∈ Γ ∧ x ≡ atom) }.
+Proof.
+  apply ZFindescr. destruct (EM (γ ∈ Γ)).
+  - exists (f γ). econstructor.
+    + apply ZFincomp. split.
+      * apply ZFinpairing. now right.
+      * left. now split.
+    + intros y Hy. apply ZFincomp in Hy. destruct Hy as [ Hy1 [ [ _ Hy2 ] | [ Hy2 _ ] ] ] ; easy.
+  - exists atom. econstructor.
+    + apply ZFincomp. split.
+      * apply ZFinpairing. now left.
+      * right. now split.
+    + intros y Hy. apply ZFincomp in Hy. destruct Hy as [ Hy1 [ [ Hy2 _ ] | [ _ Hy2 ] ] ] ; easy.
+Qed.
+
+Lemma clip_inside (Γ : ZFSet) (f : ZFSet -> ZFSet) : ∀ γ ∈ Γ, clip Γ f γ ≡ f γ.
+Proof.
+  intros γ Hγ. cbn. pose proof (clip_typing Γ f γ) as H. apply ZFincomp in H.
+  destruct H as [ H1 [ [ _ H2 ] | [ H2 _ ] ] ] ; easy.
+Qed.
+
+Lemma clip_outside (Γ : ZFSet) (f : ZFSet -> ZFSet) : forall γ, (¬ γ ∈ Γ) -> clip Γ f γ ≡ atom.
+Proof.
+  intros γ Hγ. cbn. pose proof (clip_typing Γ f γ) as H. apply ZFincomp in H.
+  destruct H as [ H1 [ [ H2 _ ] | [ _ H2 ] ] ] ; easy.
+Qed.
+
+Lemma clipped_clip (Γ : ZFSet) (f : ZFSet -> ZFSet) : is_clipped Γ (clip Γ f).
+Proof.
+  exact (clip_outside Γ f). 
+Qed.
+
+Lemma clipped_funext {Γ : ZFSet} {f g : ZFSet -> ZFSet} (Hf : is_clipped Γ f) (Hg : is_clipped Γ g) :
+  (∀ γ ∈ Γ, f γ ≡ g γ) -> f ≡ g.
+Proof.
+  intro H. apply funext. intro γ. destruct (EM (γ ∈ Γ)) as [ Hγ | Hγ ].
+  - now apply H.
+  - destruct (sym (Hf γ Hγ)). destruct (sym (Hg γ Hγ)). reflexivity.
+Qed.
+
+Lemma clip_funext (Γ : ZFSet) {f g : ZFSet -> ZFSet} :
+  (∀ γ ∈ Γ, f γ ≡ g γ) -> clip Γ f ≡ clip Γ g.
+Proof.
+  intro H. apply funext. intro γ. destruct (EM (γ ∈ Γ)) as [ Hγ | Hγ ].
+  - pose proof (sym (clip_inside Γ f γ Hγ)) as Hf. cbn in Hf. destruct Hf.
+    pose proof (sym (clip_inside Γ g γ Hγ)) as Hg. cbn in Hg. destruct Hg.
+    now apply H.
+  - pose proof (sym (clip_outside Γ f γ Hγ)) as Hf. cbn in Hf. destruct Hf.
+    pose proof (sym (clip_outside Γ g γ Hγ)) as Hg. cbn in Hg. destruct Hg.
+    reflexivity.
+Qed.
+
 (* Extended contexts *)
 
 Definition ctxExt (n : nat) (Γ : ZFSet) (A : ZFSet -> ZFSet) := setSigma n Γ (fun γ => 𝕌el n (A γ)).
 
-Definition ctx_wk (n : nat) (Γ : ZFSet) (A : ZFSet -> ZFSet) (γa : ZFSet) := setFstSigma n Γ (fun γ => 𝕌el n (A γ)) γa.
+Definition ctx_wk (n : nat) (Γ : ZFSet) (A : ZFSet -> ZFSet) (γa : ZFSet) :=
+  clip (ctxExt n Γ A) (setFstSigma n Γ (fun γ => 𝕌el n (A γ))) γa.
 
-Definition ctx_var0 (n : nat) (Γ : ZFSet) (A : ZFSet -> ZFSet) (γa : ZFSet) := setSndSigma n Γ (fun γ => 𝕌el n (A γ)) γa.
+Definition ctx_var0 (n : nat) (Γ : ZFSet) (A : ZFSet -> ZFSet) (γa : ZFSet) :=
+  clip (ctxExt n Γ A) (setSndSigma n Γ (fun γ => 𝕌el n (A γ))) γa.
 
 Lemma ctx_wk_typing {n : nat} {Γ γa : ZFSet} {A : ZFSet -> ZFSet} 
   (HA : ∀ γ ∈ Γ, A γ ∈ 𝕌 n) (Hγa : γa ∈ ctxExt n Γ A) :
   ctx_wk n Γ A γa ∈ Γ.
 Proof.
+  unfold ctx_wk. destruct (sym (clip_inside (ctxExt n Γ A) (setFstSigma n Γ (fun γ : ZFSet => 𝕌el n (A γ))) γa Hγa)).
   apply (setFstSigma_typing (A := Γ) (B := fun γ => 𝕌el n (A γ))).
   - intros γ Hγ. apply 𝕌el_typing. now apply HA.
   - assumption.
-Qed.  
+Qed.
 
 Lemma ctx_var0_typing {n : nat} {Γ γa : ZFSet} {A : ZFSet -> ZFSet} 
   (HA : ∀ γ ∈ Γ, A γ ∈ 𝕌 n) (Hγa : γa ∈ ctxExt n Γ A) :
   ctx_var0 n Γ A γa ∈ 𝕌el n (A (ctx_wk n Γ A γa)).
 Proof.
+  unfold ctx_var0. destruct (sym (clip_inside (ctxExt n Γ A) (setSndSigma n Γ (fun γ : ZFSet => 𝕌el n (A γ))) γa Hγa)).
+  unfold ctx_wk. destruct (sym (clip_inside (ctxExt n Γ A) (setFstSigma n Γ (fun γ : ZFSet => 𝕌el n (A γ))) γa Hγa)).
   apply (setSndSigma_typing (A := Γ) (B := fun γ => 𝕌el n (A γ))).
   - intros γ Hγ. apply 𝕌el_typing. now apply HA.
   - assumption.
@@ -151,6 +218,9 @@ Lemma ctxExtβ1 {n : nat} {Γ γ a : ZFSet} {A : ZFSet -> ZFSet}
   (HA : ∀ γ ∈ Γ, A γ ∈ 𝕌 n) (Hγ : γ ∈ Γ) (Ha : a ∈ 𝕌el n (A γ)) :
   ctx_wk n Γ A ⟨ γ ; a ⟩ ≡ γ.
 Proof.
+  assert (⟨ γ; a ⟩ ∈ ctxExt n Γ A) as Hγa.
+  { apply setMkSigma_typing ; try assumption. clear γ Hγ Ha. intros γ Hγ. apply 𝕌el_typing. now apply HA. }
+  unfold ctx_wk. destruct (sym (clip_inside (ctxExt n Γ A) (setFstSigma n Γ (fun γ : ZFSet => 𝕌el n (A γ))) _ Hγa)).
   apply (setSigmaβ1 (A := Γ) (B := fun γ => 𝕌el n (A γ))) ; try assumption.
   intros γ' Hγ'. apply 𝕌el_typing. now apply HA.
 Qed.
@@ -159,6 +229,9 @@ Lemma ctxExtβ2 {n : nat} {Γ γ a : ZFSet} {A : ZFSet -> ZFSet}
   (HA : ∀ γ ∈ Γ, A γ ∈ 𝕌 n) (Hγ : γ ∈ Γ) (Ha : a ∈ 𝕌el n (A γ)) :
   ctx_var0 n Γ A ⟨ γ ; a ⟩ ≡ a.
 Proof.
+  assert (⟨ γ; a ⟩ ∈ ctxExt n Γ A) as Hγa.
+  { apply setMkSigma_typing ; try assumption. clear γ Hγ Ha. intros γ Hγ. apply 𝕌el_typing. now apply HA. }
+  unfold ctx_var0. destruct (sym (clip_inside (ctxExt n Γ A) (setSndSigma n Γ (fun γ : ZFSet => 𝕌el n (A γ))) _ Hγa)).
   apply (setSigmaβ2 (A := Γ) (B := fun γ => 𝕌el n (A γ))) ; try assumption.
   intros γ' Hγ'. apply 𝕌el_typing. now apply HA.
 Qed.
@@ -237,51 +310,7 @@ Proof.
     + apply typeToGraph_sorting. now apply HA. now apply (typeExt_typing HA HB).
 Qed.
 
-(* Restricting the domain of higher-order functions to get funext *)
-(* Requires excluded middle! *)
-
-Definition clip (Γ : ZFSet) (f : ZFSet -> ZFSet) : ZFSet -> ZFSet :=
-  fun γ => ι { x ϵ { ∅ ; f γ } ∣ (γ ∈ Γ ∧ x ≡ f γ) ∨ (¬ γ ∈ Γ ∧ x ≡ ∅) }.
-
-Lemma clip_typing (Γ : ZFSet) (f : ZFSet -> ZFSet) (γ : ZFSet) :
-  clip Γ f γ ∈ { x ϵ { ∅ ; f γ } ∣ (γ ∈ Γ ∧ x ≡ f γ) ∨ (¬ γ ∈ Γ ∧ x ≡ ∅) }.
-Proof.
-  apply ZFindescr. destruct (EM (γ ∈ Γ)).
-  - exists (f γ). econstructor.
-    + apply ZFincomp. split.
-      * apply ZFinpairing. now right.
-      * left. now split.
-    + intros y Hy. apply ZFincomp in Hy. destruct Hy as [ Hy1 [ [ _ Hy2 ] | [ Hy2 _ ] ] ] ; easy.
-  - exists ∅. econstructor.
-    + apply ZFincomp. split.
-      * apply ZFinpairing. now left.
-      * right. now split.
-    + intros y Hy. apply ZFincomp in Hy. destruct Hy as [ Hy1 [ [ Hy2 _ ] | [ _ Hy2 ] ] ] ; easy.
-Qed.
-
-Lemma clip_inside (Γ : ZFSet) (f : ZFSet -> ZFSet) : ∀ γ ∈ Γ, clip Γ f γ ≡ f γ.
-Proof.
-  intros γ Hγ. cbn. pose proof (clip_typing Γ f γ) as H. apply ZFincomp in H.
-  destruct H as [ H1 [ [ _ H2 ] | [ H2 _ ] ] ] ; easy.
-Qed.
-
-Lemma clip_outside (Γ : ZFSet) (f : ZFSet -> ZFSet) : forall γ, (¬ γ ∈ Γ) -> clip Γ f γ ≡ ∅.
-Proof.
-  intros γ Hγ. cbn. pose proof (clip_typing Γ f γ) as H. apply ZFincomp in H.
-  destruct H as [ H1 [ [ H2 _ ] | [ _ H2 ] ] ] ; easy.
-Qed.
-
-Lemma clip_funext (Γ : ZFSet) {f g : ZFSet -> ZFSet} :
-  (∀ γ ∈ Γ, f γ ≡ g γ) -> clip Γ f ≡ clip Γ g.
-Proof.
-  intro H. apply funext. intro γ. destruct (EM (γ ∈ Γ)) as [ Hγ | Hγ ].
-  - pose proof (sym (clip_inside Γ f γ Hγ)) as Hf. cbn in Hf. destruct Hf.
-    pose proof (sym (clip_inside Γ g γ Hγ)) as Hg. cbn in Hg. destruct Hg.
-    now apply H.
-  - pose proof (sym (clip_outside Γ f γ Hγ)) as Hf. cbn in Hf. destruct Hf.
-    pose proof (sym (clip_outside Γ g γ Hγ)) as Hg. cbn in Hg. destruct Hg.
-    reflexivity.
-Qed.
+(* Tools for clipping *)
 
 Lemma clipped_typing_𝕌 {n : nat} (Γ : ZFSet) (t : ZFSet -> ZFSet) :
   (∀ γ ∈ Γ, t γ ∈ 𝕌 n) -> (∀ γ ∈ Γ, clip Γ t γ ∈ 𝕌 n).
@@ -312,13 +341,17 @@ Qed.
 Lemma clipped_wk (n : nat) (Γ : ZFSet) (A : ZFSet -> ZFSet) (γa : ZFSet) :
   ctx_wk n Γ (clip Γ A) γa ≡ ctx_wk n Γ A γa.
 Proof.
-  unfold ctx_wk. unfold setFstSigma. refine (fequal (fun X => setFstPair Γ X γa) _).
+  unfold ctx_wk. destruct (sym (clipped_ext n Γ A)). refine (fequal (fun X => X γa) _).
+  clear γa. apply clip_funext. intros γa Hγa. unfold setFstSigma.
+  refine (fequal (fun X => setFstPair Γ X γa) _).
   apply setFamUnion_cong. intros γ Hγ. destruct (sym (clip_inside Γ A γ Hγ)). reflexivity.
 Qed.
 
 Lemma clipped_var0 (n : nat) (Γ : ZFSet) (A : ZFSet -> ZFSet) (γa : ZFSet) :
   ctx_var0 n Γ (clip Γ A) γa ≡ ctx_var0 n Γ A γa.
 Proof.
-  unfold ctx_wk. unfold setSndSigma. refine (fequal (fun X => setSndPair Γ X γa) _).
+  unfold ctx_var0. destruct (sym (clipped_ext n Γ A)). refine (fequal (fun X => X γa) _).
+  clear γa. apply clip_funext. intros γa Hγa. unfold setSndSigma.
+  refine (fequal (fun X => setSndPair Γ X γa) _).
   apply setFamUnion_cong. intros γ Hγ. destruct (sym (clip_inside Γ A γ Hγ)). reflexivity.
 Qed.
