theories/SetModel/HO_prop.v
@@ -30,3 +30,17 @@ Proof.
   intros γ Hγ. specialize (HP γ Hγ). specialize (Hp γ Hγ). specialize (Hq γ Hγ). cbn in *.
   refine (trans _ (sym _)). now apply (proof_irr HP). now apply (proof_irr HP).
 Qed.
+
+(* Clipped version *)
+
+Definition propTy_cl (Γ : ZFSet) : ZFSet -> ZFSet := clip Γ propTy_HO.
+
+Lemma propTy_cl_typing {n : nat} {Γ : ZFSet} : ∀ γ ∈ Γ, propTy_cl Γ γ ∈ 𝕌 n.
+Proof.
+  apply clipped_typing_𝕌. now apply propTy_HO_typing.
+Qed.
+
+Lemma el_propTy_cl {n : nat} {Γ γ : ZFSet} (Hγ : γ ∈ Γ) : 𝕌el n (propTy_cl Γ γ) ≡ Ω.
+Proof.
+  unfold propTy_cl. destruct (sym (clip_inside Γ propTy_HO γ Hγ)). now apply el_propTy.
+Qed.
